\begin{eqnarray*}
\sum_{i=1}^ni^1=&\frac{n(n+1)}{2}=\frac{1}{2}n^2+\frac{1}{2}n\\
\sum_{i=1}^ni^2=&\frac{n(n+1)(2n+1)}{6}=\frac{1}{3}n^3+\frac{1}{2}n^2+\frac{1}{6}n\\
\sum_{i=1}^ni^3=&\left[\frac{n(n+1)}{2}\right]^2=\frac{1}{4}n^4+\frac{1}{2}n^3+\frac{1}{4}n^2\\
\sum_{i=1}^ni^4=&\frac{n(n+1)(2n+1)(3n^2+3n-1)}{30}\\=&\frac{1}{5}n^5+\frac{1}{2}n^4+\frac{1}{3}n^3-\frac{1}{30}n\\
\sum_{i=1}^ni^5=&\frac{n^2(n+1)^2(2n^2+2n-1)}{12}\\=&\frac{1}{6}n^6+\frac{1}{2}n^5+\frac{5}{12}n^4-\frac{1}{12}n^2\\
\sum_{i=1}^ni^6=&\frac{n(n+1)(2n+1)(3n^4+6n^3-3n+1)}{42}\\=&\frac{1}{7}n^7+\frac{1}{2}n^6+\frac{1}{2}n^5-\frac{1}{6}n^3+\frac{1}{42}n
\end{eqnarray*}
